concurrency/disciplined/Impl.i.dfy
@@ -42,8 +42,8 @@ module Impl refines VerificationObligation {
     requires r.tickets == multiset{}
     requires r.stubs == multiset{}
   {
-    var r' := SSM.Variables(seq(|r.table|, (j) requires 0<=j<|r.table| => if j!=i then r.table[j] else None), r.insert_capacity, multiset{}, multiset{});
-    var ri := SSM.Variables(seq(|r.table|, (j) requires 0<=j<|r.table| => if j==i then r.table[j] else None), 0, multiset{}, multiset{});
+    var r' := SSM.Variables(seq(|r.table|, (j) requires 0 <= j < |r.table| => if j!=i then r.table[j] else None), r.insert_capacity, multiset{}, multiset{});
+    var ri := SSM.Variables(seq(|r.table|, (j) requires 0 <= j < |r.table| => if j==i then r.table[j] else None), Count.Variables(0), multiset{}, multiset{});
     Splitted(r', ri)
   }
 
@@ -64,7 +64,7 @@ module Impl refines VerificationObligation {
       invariant remaining_r.stubs == multiset{} 
       invariant forall k:nat | k < i as int :: remaining_r.table[k].None?
       invariant forall l:nat | i as int <= l < |remaining_r.table| :: remaining_r.table[l] == Some(Info(Empty, Free))
-      invariant remaining_r.insert_capacity == Capacity()
+      invariant remaining_r.insert_capacity.value == Capacity()
     {
       ghost var splitted := Split(remaining_r, i as int);
       glinear var ri;
@@ -74,540 +74,537 @@ module Impl refines VerificationObligation {
       i := i + 1;
     }
 
-    var allocator: CAP.AllocatorMutexTable;
-    allocator, out_sv := CAP.init(remaining_r);
-
-    v := Variables.Variables(row_mutexes, allocator);
-
-    assert forall i:nat | i < FixedSize() :: out_sv.table[i].None?;
-    assert out_sv == unit();
+    assert remaining_r.table == unitTable();
+    glinear var insert_capacity;
+    out_sv, insert_capacity := declose(remaining_r);
+    init(insert_capacity);
   }
 
-  predicate method shouldHashGoBefore(search_h: uint32, slot_h: uint32, slot_idx: uint32) 
-    ensures shouldHashGoBefore(search_h, slot_h, slot_idx) == ShouldHashGoBefore(search_h as int, slot_h as int, slot_idx as int)
-  {
-    || search_h < slot_h <= slot_idx // normal case
-    || slot_h <= slot_idx < search_h // search_h wraps around the end of array
-    || slot_idx < search_h < slot_h// search_h, slot_h wrap around the end of array
-  }
+  // predicate method shouldHashGoBefore(search_h: uint32, slot_h: uint32, slot_idx: uint32) 
+  //   ensures shouldHashGoBefore(search_h, slot_h, slot_idx) == ShouldHashGoBefore(search_h as int, slot_h as int, slot_idx as int)
+  // {
+  //   || search_h < slot_h <= slot_idx // normal case
+  //   || slot_h <= slot_idx < search_h // search_h wraps around the end of array
+  //   || slot_idx < search_h < slot_h// search_h, slot_h wrap around the end of array
+  // }
 
-  function method getNextIndex(slot_idx: uint32) : uint32
-    requires slot_idx < FixedSizeImpl()
-  {
-    if slot_idx == FixedSizeImpl() - 1 then 0 else slot_idx + 1
-  }
+  // function method getNextIndex(slot_idx: uint32) : uint32
+  //   requires slot_idx < FixedSizeImpl()
+  // {
+  //   if slot_idx == FixedSizeImpl() - 1 then 0 else slot_idx + 1
+  // }
 
-  function DistanceToSlot(src: uint32, dst: uint32) : nat
-    requires src < FixedSizeImpl()
-    requires dst < FixedSizeImpl()
-  {
-    if src >= dst
-      then (dst as int - src as int + FixedSize() as int)
-      else (dst as int - src as int)
-  }
+  // function DistanceToSlot(src: uint32, dst: uint32) : nat
+  //   requires src < FixedSizeImpl()
+  //   requires dst < FixedSizeImpl()
+  // {
+  //   if src >= dst
+  //     then (dst as int - src as int + FixedSize() as int)
+  //     else (dst as int - src as int)
+  // }
 
-  method doQuery(v: Variables, input: Ifc.Input, rid: int, glinear in_sv: SSM.Variables)
-  returns (output: Ifc.Output, glinear out_sv: SSM.Variables)
-    decreases *
-    requires Inv(v)
-    requires input.QueryInput?
-    requires isInputResource(in_sv, rid, input)
-    ensures out_sv == SSM.output_stub(rid, output)
-  {
-    var query_ticket := Ticket(rid, input);
-    var key := input.key;
-    var hash_idx := hash(key);
-    var slot_idx := hash_idx;
+  // method doQuery(v: Variables, input: Ifc.Input, rid: int, glinear in_sv: SSM.Variables)
+  // returns (output: Ifc.Output, glinear out_sv: SSM.Variables)
+  //   decreases *
+  //   requires Inv(v)
+  //   requires input.QueryInput?
+  //   requires isInputResource(in_sv, rid, input)
+  //   ensures out_sv == SSM.output_stub(rid, output)
+  // {
+  //   var query_ticket := Ticket(rid, input);
+  //   var key := input.key;
+  //   var hash_idx := hash(key);
+  //   var slot_idx := hash_idx;
 
-    linear var row; glinear var handle;
-    row, handle := v.row_mutexes[slot_idx].acquire();
-    linear var Row(entry, row_r) := row;
-    glinear var r := SSM.join(in_sv, row_r);
+  //   linear var row; glinear var handle;
+  //   row, handle := v.row_mutexes[slot_idx].acquire();
+  //   linear var Row(entry, row_r) := row;
+  //   glinear var r := SSM.join(in_sv, row_r);
 
-    ghost var r' := oneRowResource(hash_idx as nat, Info(entry, Querying(rid, key)), 0);
-    assert ProcessQueryTicket(r, r', query_ticket);
+  //   ghost var r' := oneRowResource(hash_idx as nat, Info(entry, Querying(rid, key)), 0);
+  //   assert ProcessQueryTicket(r, r', query_ticket);
 
-    var step := ProcessQueryTicketStep(query_ticket);
-    r := easy_transform_step(r, r', step);
+  //   var step := ProcessQueryTicketStep(query_ticket);
+  //   r := easy_transform_step(r, r', step);
 
-    while true 
-      invariant Inv(v);
-      invariant 0 <= slot_idx < FixedSizeImpl();
-      invariant r == oneRowResource(slot_idx as nat, Info(entry, Querying(rid, key)), 0);
-      invariant handle.m == v.row_mutexes[slot_idx];
-      decreases *
-    {
-      var slot_idx' := getNextIndex(slot_idx);
+  //   while true 
+  //     invariant Inv(v);
+  //     invariant 0 <= slot_idx < FixedSizeImpl();
+  //     invariant r == oneRowResource(slot_idx as nat, Info(entry, Querying(rid, key)), 0);
+  //     invariant handle.m == v.row_mutexes[slot_idx];
+  //     decreases *
+  //   {
+  //     var slot_idx' := getNextIndex(slot_idx);
 
-      match entry {
-        case Empty => {
-          output := MapIfc.QueryOutput(NotFound);
-          step := QueryNotFoundStep(slot_idx as nat);
-        }
-        case Full(KV(entry_key, value)) => {
-          if entry_key == key {
-            step := QueryDoneStep(slot_idx as nat);
-            output := MapIfc.QueryOutput(Found(value));
-          } else {
-            var should_go_before := shouldHashGoBefore(hash_idx, hash(entry_key), slot_idx);
+  //     match entry {
+  //       case Empty => {
+  //         output := MapIfc.QueryOutput(NotFound);
+  //         step := QueryNotFoundStep(slot_idx as nat);
+  //       }
+  //       case Full(KV(entry_key, value)) => {
+  //         if entry_key == key {
+  //           step := QueryDoneStep(slot_idx as nat);
+  //           output := MapIfc.QueryOutput(Found(value));
+  //         } else {
+  //           var should_go_before := shouldHashGoBefore(hash_idx, hash(entry_key), slot_idx);
 
-            if !should_go_before {
-              step := QuerySkipStep(slot_idx as nat);
-            } else {
-              output := MapIfc.QueryOutput(NotFound);
-              step := QueryNotFoundStep(slot_idx as nat);
-            }
-          }
-        }
-      }
+  //           if !should_go_before {
+  //             step := QuerySkipStep(slot_idx as nat);
+  //           } else {
+  //             output := MapIfc.QueryOutput(NotFound);
+  //             step := QueryNotFoundStep(slot_idx as nat);
+  //           }
+  //         }
+  //       }
+  //     }
 
-      if !step.QuerySkipStep? {
-        // this test is required for termination, but is not enforced by verification
-        // because we are using decreases *
-        break;
-      }
+  //     if !step.QuerySkipStep? {
+  //       // this test is required for termination, but is not enforced by verification
+  //       // because we are using decreases *
+  //       break;
+  //     }
 
-      // if slot_idx' == hash_idx {
-      //   QueryUnreachableState(r, slot_idx as nat);
-      //   break;
-      // }
+  //     // if slot_idx' == hash_idx {
+  //     //   QueryUnreachableState(r, slot_idx as nat);
+  //     //   break;
+  //     // }
 
-      linear var next_row; glinear var next_handle;
-      next_row, next_handle := v.row_mutexes[slot_idx'].acquire();
-      linear var Row(next_entry, next_row_r) := next_row;
-      r := SSM.join(r, next_row_r);
+  //     linear var next_row; glinear var next_handle;
+  //     next_row, next_handle := v.row_mutexes[slot_idx'].acquire();
+  //     linear var Row(next_entry, next_row_r) := next_row;
+  //     r := SSM.join(r, next_row_r);
 
-      r' := twoRowsResource(slot_idx as nat, Info(entry, Free), slot_idx' as nat, Info(next_entry, Querying(rid, key)), 0);
-      r := easy_transform_step(r, r', step);
+  //     r' := twoRowsResource(slot_idx as nat, Info(entry, Free), slot_idx' as nat, Info(next_entry, Querying(rid, key)), 0);
+  //     r := easy_transform_step(r, r', step);
 
-      glinear var rmutex;
-      ghost var left := oneRowResource(slot_idx' as nat, Info(next_entry, Querying(rid, key)), 0);
-      ghost var right := oneRowResource(slot_idx as nat, Info(entry, Free), 0);
-      r, rmutex := SSM.split(r, left, right);
-      v.row_mutexes[slot_idx].release(Row(entry, rmutex), handle);
+  //     glinear var rmutex;
+  //     ghost var left := oneRowResource(slot_idx' as nat, Info(next_entry, Querying(rid, key)), 0);
+  //     ghost var right := oneRowResource(slot_idx as nat, Info(entry, Free), 0);
+  //     r, rmutex := SSM.split(r, left, right);
+  //     v.row_mutexes[slot_idx].release(Row(entry, rmutex), handle);
 
-      slot_idx := slot_idx';
-      entry := next_entry;
-      handle := next_handle;
-    }
+  //     slot_idx := slot_idx';
+  //     entry := next_entry;
+  //     handle := next_handle;
+  //   }
     
-    // assert step.QueryNotFoundStep? || step.QueryDoneStep?;
-    r' := SSM.Variables(oneRowTable(slot_idx as nat, Info(entry, Free)), 0, multiset{}, multiset{Stub(rid, output)}); 
-    r := easy_transform_step(r, r', step);
+  //   // assert step.QueryNotFoundStep? || step.QueryDoneStep?;
+  //   r' := SSM.Variables(oneRowTable(slot_idx as nat, Info(entry, Free)), 0, multiset{}, multiset{Stub(rid, output)}); 
+  //   r := easy_transform_step(r, r', step);
 
-    glinear var rmutex;
-    r, rmutex := SSM.split(r, 
-      SSM.output_stub(rid, output), 
-      oneRowResource(slot_idx as nat, Info(entry, Free), 0));
-    v.row_mutexes[slot_idx].release(Row(entry, rmutex), handle);
+  //   glinear var rmutex;
+  //   r, rmutex := SSM.split(r, 
+  //     SSM.output_stub(rid, output), 
+  //     oneRowResource(slot_idx as nat, Info(entry, Free), 0));
+  //   v.row_mutexes[slot_idx].release(Row(entry, rmutex), handle);
 
-    out_sv := r;
-  }
+  //   out_sv := r;
+  // }
 
-  method acquireCapacity(v: Variables, thread_id: uint32)
-  returns (linear cap: AllocatorBin, glinear cap_handle: MutexHandle<AllocatorBin>, tid: uint32)
-    decreases *
-    requires Inv(v)
-    ensures cap.resource == unit().(insert_capacity := cap.count as nat)
-    ensures 0 < cap.count
-    ensures tid < CAP.BinCountImpl()
-    ensures cap_handle.m == v.allocator[tid]
-  {
-    // thread_id is a hint for the bin we're supposed to use. 
-    // tid is the actual place we found the capacity (in case we had to steal it from someone else) 
-    tid := if thread_id >= CAP.BinCountImpl() then 0 else thread_id;
-    cap, cap_handle := v.allocator[tid].acquire();
+  // method acquireCapacity(v: Variables, thread_id: uint32)
+  // returns (linear cap: AllocatorBin, glinear cap_handle: MutexHandle<AllocatorBin>, tid: uint32)
+  //   decreases *
+  //   requires Inv(v)
+  //   ensures cap.resource == unit().(insert_capacity := cap.count as nat)
+  //   ensures 0 < cap.count
+  //   ensures tid < CAP.BinCountImpl()
+  //   ensures cap_handle.m == v.allocator[tid]
+  // {
+  //   // thread_id is a hint for the bin we're supposed to use. 
+  //   // tid is the actual place we found the capacity (in case we had to steal it from someone else) 
+  //   tid := if thread_id >= CAP.BinCountImpl() then 0 else thread_id;
+  //   cap, cap_handle := v.allocator[tid].acquire();
 
-    while true
-      invariant tid < CAP.BinCountImpl()
-      invariant cap.resource == unit().(insert_capacity := cap.count as nat)
-      invariant cap_handle.m == v.allocator[tid]
-      decreases *
-    {
-      if 0 < cap.count {
-        break;
-      }
+  //   while true
+  //     invariant tid < CAP.BinCountImpl()
+  //     invariant cap.resource == unit().(insert_capacity := cap.count as nat)
+  //     invariant cap_handle.m == v.allocator[tid]
+  //     decreases *
+  //   {
+  //     if 0 < cap.count {
+  //       break;
+  //     }
 
-      // assert exists s' :: TableQuantityInv(add(s, s'))
-      assert CAP.BinInv(cap);
-      v.allocator[tid].release(cap, cap_handle);
+  //     // assert exists s' :: TableQuantityInv(add(s, s'))
+  //     assert CAP.BinInv(cap);
+  //     v.allocator[tid].release(cap, cap_handle);
 
-      tid := tid + 1;
-      tid := if tid >= CAP.BinCountImpl() then 0 else tid;
+  //     tid := tid + 1;
+  //     tid := if tid >= CAP.BinCountImpl() then 0 else tid;
 
-      cap, cap_handle := v.allocator[tid].acquire();
-    }
-  }
+  //     cap, cap_handle := v.allocator[tid].acquire();
+  //   }
+  // }
 
-  method doInsert(v: Variables, input: Ifc.Input, rid: int, thread_id: uint32, glinear in_sv: SSM.Variables)
-  returns (output: Ifc.Output, glinear out_sv: SSM.Variables)
-    requires Inv(v)
-    requires input.InsertInput?
-    requires isInputResource(in_sv, rid, input)
-    ensures out_sv == SSM.output_stub(rid, output)
-    decreases *
-  {
-    var allocator := v.allocator;
+  // method doInsert(v: Variables, input: Ifc.Input, rid: int, thread_id: uint32, glinear in_sv: SSM.Variables)
+  // returns (output: Ifc.Output, glinear out_sv: SSM.Variables)
+  //   requires Inv(v)
+  //   requires input.InsertInput?
+  //   requires isInputResource(in_sv, rid, input)
+  //   ensures out_sv == SSM.output_stub(rid, output)
+  //   decreases *
+  // {
+  //   var allocator := v.allocator;
 
-    var query_ticket := Ticket(rid, input);
-    var key, inital_key := input.key, input.key;
-    var kv := KV(key, input.value);
-    output := MapIfc.InsertOutput(true);
+  //   var query_ticket := Ticket(rid, input);
+  //   var key, inital_key := input.key, input.key;
+  //   var kv := KV(key, input.value);
+  //   output := MapIfc.InsertOutput(true);
 
-    var hash_idx := hash(key);
-    var initial_hash_idx := hash_idx;
-    var slot_idx := hash_idx;
+  //   var hash_idx := hash(key);
+  //   var initial_hash_idx := hash_idx;
+  //   var slot_idx := hash_idx;
 
-    linear var cap; glinear var cap_handle; var tid;
-    cap, cap_handle, tid := acquireCapacity(v, thread_id);
-    linear var AllocatorBin(count, cap_r) := cap;
-    glinear var r := SSM.join(in_sv, cap_r);
+  //   linear var cap; glinear var cap_handle; var tid;
+  //   cap, cap_handle, tid := acquireCapacity(v, thread_id);
+  //   linear var AllocatorBin(count, cap_r) := cap;
+  //   glinear var r := SSM.join(in_sv, cap_r);
 
-    linear var row; glinear var handle;
-    row, handle := v.row_mutexes[slot_idx].acquire();
-    linear var Row(entry, row_r) := row;
-    r := SSM.join(r, row_r);
+  //   linear var row; glinear var handle;
+  //   row, handle := v.row_mutexes[slot_idx].acquire();
+  //   linear var Row(entry, row_r) := row;
+  //   r := SSM.join(r, row_r);
 
-    count := count - 1;
+  //   count := count - 1;
 
-    var step := ProcessInsertTicketStep(query_ticket);
-    ghost var r' := oneRowResource(hash_idx as nat, Info(entry, Inserting(rid, kv, inital_key)), count as nat);
-    r := easy_transform_step(r, r', step);
-    glinear var rmutex;
+  //   var step := ProcessInsertTicketStep(query_ticket);
+  //   ghost var r' := oneRowResource(hash_idx as nat, Info(entry, Inserting(rid, kv, inital_key)), count as nat);
+  //   r := easy_transform_step(r, r', step);
+  //   glinear var rmutex;
 
-    while true 
-      invariant Inv(v);
-      invariant 0 <= slot_idx < FixedSizeImpl()
-      invariant r == oneRowResource(slot_idx as nat, Info(entry, Inserting(rid, kv, inital_key)), count as nat)
-      invariant kv.key == key
-      invariant hash_idx == hash(key)
-      invariant handle.m == v.row_mutexes[slot_idx];
-      decreases *
-    {
-      var slot_idx' := getNextIndex(slot_idx);
-      var new_kv;
+  //   while true 
+  //     invariant Inv(v);
+  //     invariant 0 <= slot_idx < FixedSizeImpl()
+  //     invariant r == oneRowResource(slot_idx as nat, Info(entry, Inserting(rid, kv, inital_key)), count as nat)
+  //     invariant kv.key == key
+  //     invariant hash_idx == hash(key)
+  //     invariant handle.m == v.row_mutexes[slot_idx];
+  //     decreases *
+  //   {
+  //     var slot_idx' := getNextIndex(slot_idx);
+  //     var new_kv;
 
-      match entry {
-        case Empty => {
-          step := InsertDoneStep(slot_idx as nat);
-        }
-        case Full(KV(entry_key, value)) => {
-          new_kv := KV(entry_key, value);
-          if entry_key == key {
-            step := InsertUpdateStep(slot_idx as nat);
-          } else {
-            var should_go_before := shouldHashGoBefore(hash_idx, hash(entry_key), slot_idx);
-            if !should_go_before {
-              step := InsertSkipStep(slot_idx as nat);
-            } else {
-              step := InsertSwapStep(slot_idx as nat);
-            }
-          }
-        }
-      }
+  //     match entry {
+  //       case Empty => {
+  //         step := InsertDoneStep(slot_idx as nat);
+  //       }
+  //       case Full(KV(entry_key, value)) => {
+  //         new_kv := KV(entry_key, value);
+  //         if entry_key == key {
+  //           step := InsertUpdateStep(slot_idx as nat);
+  //         } else {
+  //           var should_go_before := shouldHashGoBefore(hash_idx, hash(entry_key), slot_idx);
+  //           if !should_go_before {
+  //             step := InsertSkipStep(slot_idx as nat);
+  //           } else {
+  //             step := InsertSwapStep(slot_idx as nat);
+  //           }
+  //         }
+  //       }
+  //     }
 
-      if step.InsertDoneStep? || step.InsertUpdateStep? {
-        break;
-      }
+  //     if step.InsertDoneStep? || step.InsertUpdateStep? {
+  //       break;
+  //     }
 
-      linear var next_row; glinear var next_handle;
-      next_row, next_handle := v.row_mutexes[slot_idx'].acquire();
-      linear var Row(next_entry, next_row_r) := next_row;
-      r := SSM.join(r, next_row_r);
+  //     linear var next_row; glinear var next_handle;
+  //     next_row, next_handle := v.row_mutexes[slot_idx'].acquire();
+  //     linear var Row(next_entry, next_row_r) := next_row;
+  //     r := SSM.join(r, next_row_r);
 
-      if step.InsertSwapStep? {
-        entry := Full(kv);
-        kv := new_kv;
-        key := new_kv.key;
-      }
+  //     if step.InsertSwapStep? {
+  //       entry := Full(kv);
+  //       kv := new_kv;
+  //       key := new_kv.key;
+  //     }
   
-      r' := twoRowsResource(slot_idx as nat, Info(entry, Free), slot_idx' as nat, Info(next_entry, Inserting(rid, kv, inital_key)), count as nat);
-      r := easy_transform_step(r, r', step);
+  //     r' := twoRowsResource(slot_idx as nat, Info(entry, Free), slot_idx' as nat, Info(next_entry, Inserting(rid, kv, inital_key)), count as nat);
+  //     r := easy_transform_step(r, r', step);
 
-      ghost var left := oneRowResource(slot_idx' as nat, Info(next_entry, Inserting(rid, kv, inital_key)), count as nat);
-      ghost var right := oneRowResource(slot_idx as nat, Info(entry, Free), 0);
+  //     ghost var left := oneRowResource(slot_idx' as nat, Info(next_entry, Inserting(rid, kv, inital_key)), count as nat);
+  //     ghost var right := oneRowResource(slot_idx as nat, Info(entry, Free), 0);
 
-      r, rmutex := SSM.split(r, left, right);
-      v.row_mutexes[slot_idx].release(Row(entry, rmutex), handle);
+  //     r, rmutex := SSM.split(r, left, right);
+  //     v.row_mutexes[slot_idx].release(Row(entry, rmutex), handle);
 
-      slot_idx := slot_idx';
-      entry := next_entry;
-      hash_idx := hash(key);
-      handle := next_handle;
-    }
+  //     slot_idx := slot_idx';
+  //     entry := next_entry;
+  //     hash_idx := hash(key);
+  //     handle := next_handle;
+  //   }
 
-    // assert step.InsertDoneStep? || step.InsertUpdateStep?;
-    count := if step.InsertDoneStep? then count else count + 1;
-    r' := SSM.Variables(oneRowTable(slot_idx as nat, Info(Full(kv), Free)), count as nat, multiset{}, multiset{Stub(rid, output)});
-    r := easy_transform_step(r, r', step);
+  //   // assert step.InsertDoneStep? || step.InsertUpdateStep?;
+  //   count := if step.InsertDoneStep? then count else count + 1;
+  //   r' := SSM.Variables(oneRowTable(slot_idx as nat, Info(Full(kv), Free)), count as nat, multiset{}, multiset{Stub(rid, output)});
+  //   r := easy_transform_step(r, r', step);
 
-    r, rmutex := SSM.split(r, 
-      SSM.output_stub(rid, output).(insert_capacity := count as nat), 
-      oneRowResource(slot_idx as nat, Info(Full(kv), Free), 0));
-    v.row_mutexes[slot_idx].release(Row(Full(kv), rmutex), handle);
+  //   r, rmutex := SSM.split(r, 
+  //     SSM.output_stub(rid, output).(insert_capacity := count as nat), 
+  //     oneRowResource(slot_idx as nat, Info(Full(kv), Free), 0));
+  //   v.row_mutexes[slot_idx].release(Row(Full(kv), rmutex), handle);
 
-    glinear var rcap;
-    r, rcap := SSM.split(r,
-      SSM.output_stub(rid, output), 
-      unit().(insert_capacity := count as nat));
+  //   glinear var rcap;
+  //   r, rcap := SSM.split(r,
+  //     SSM.output_stub(rid, output), 
+  //     unit().(insert_capacity := count as nat));
 
-    assert CAP.BinInv(AllocatorBin(count, rcap)); // ha ha ha
-    allocator[tid].release(AllocatorBin(count, rcap), cap_handle);
+  //   assert CAP.BinInv(AllocatorBin(count, rcap)); // ha ha ha
+  //   allocator[tid].release(AllocatorBin(count, rcap), cap_handle);
 
-    out_sv := r;
-  }
+  //   out_sv := r;
+  // }
 
-  method doRemoveFound(v: Variables, rid: int, 
-    slot_idx: uint32,
-    hash_idx: uint32,
-    inital_key: Key,
-    entry: SSM.Entry,
-    thread_id: uint32,
-    glinear handle: MutexHandle<Row>,
-    glinear r: SSM.Variables)
+  // method doRemoveFound(v: Variables, rid: int, 
+  //   slot_idx: uint32,
+  //   hash_idx: uint32,
+  //   inital_key: Key,
+  //   entry: SSM.Entry,
+  //   thread_id: uint32,
+  //   glinear handle: MutexHandle<Row>,
+  //   glinear r: SSM.Variables)
   
-    returns (output: Ifc.Output, glinear out_sv: SSM.Variables)
-    decreases *
-    requires Inv(v)
-    requires 0 <= slot_idx < FixedSizeImpl()
-    requires 0 <= hash_idx < FixedSizeImpl()
-    requires r == oneRowResource(slot_idx as nat, Info(entry, Removing(rid, inital_key)), 0);
-    requires entry.Full? && entry.kv.key == inital_key
-    requires hash(inital_key) == hash_idx
-    requires handle.m == v.row_mutexes[slot_idx]
-    ensures out_sv == SSM.output_stub(rid, output)
-  {
-    var found_value := entry.kv.val;
-    // var allocator := v.allocator;
+  //   returns (output: Ifc.Output, glinear out_sv: SSM.Variables)
+  //   decreases *
+  //   requires Inv(v)
+  //   requires 0 <= slot_idx < FixedSizeImpl()
+  //   requires 0 <= hash_idx < FixedSizeImpl()
+  //   requires r == oneRowResource(slot_idx as nat, Info(entry, Removing(rid, inital_key)), 0);
+  //   requires entry.Full? && entry.kv.key == inital_key
+  //   requires hash(inital_key) == hash_idx
+  //   requires handle.m == v.row_mutexes[slot_idx]
+  //   ensures out_sv == SSM.output_stub(rid, output)
+  // {
+  //   var found_value := entry.kv.val;
+  //   // var allocator := v.allocator;
 
-    var slot_idx := slot_idx;
-    var slot_idx' := getNextIndex(slot_idx);
+  //   var slot_idx := slot_idx;
+  //   var slot_idx' := getNextIndex(slot_idx);
 
-    glinear var handle := handle;
-    glinear var rmutex;
+  //   glinear var handle := handle;
+  //   glinear var rmutex;
 
-    linear var next_row; glinear var next_handle;
-    next_row, next_handle := v.row_mutexes[slot_idx'].acquire();
-    linear var Row(next_entry, next_row_r) := next_row;
-    glinear var r := SSM.join(r, next_row_r);
+  //   linear var next_row; glinear var next_handle;
+  //   next_row, next_handle := v.row_mutexes[slot_idx'].acquire();
+  //   linear var Row(next_entry, next_row_r) := next_row;
+  //   glinear var r := SSM.join(r, next_row_r);
 
-    var step := RemoveFoundItStep(slot_idx as nat);
-    var r' := twoRowsResource(
-        slot_idx as nat, Info(Empty, RemoveTidying(rid, inital_key, found_value)),
-        slot_idx' as nat, Info(next_entry, Free),
-        0);
-    r := easy_transform_step(r, r', step);
+  //   var step := RemoveFoundItStep(slot_idx as nat);
+  //   var r' := twoRowsResource(
+  //       slot_idx as nat, Info(Empty, RemoveTidying(rid, inital_key, found_value)),
+  //       slot_idx' as nat, Info(next_entry, Free),
+  //       0);
+  //   r := easy_transform_step(r, r', step);
 
-    while true
-      invariant Inv(v);
-      invariant 0 <= slot_idx < FixedSizeImpl()
-      invariant r == twoRowsResource(
-        slot_idx as nat, Info(Empty, RemoveTidying(rid, inital_key, found_value)),
-        NextPos(slot_idx as nat), Info(next_entry, Free),
-        0)
-      invariant handle.m == v.row_mutexes[slot_idx]
-      invariant next_handle.m == v.row_mutexes[NextPos(slot_idx as nat)]
-      decreases *
-    {
-      slot_idx' := getNextIndex(slot_idx);
+  //   while true
+  //     invariant Inv(v);
+  //     invariant 0 <= slot_idx < FixedSizeImpl()
+  //     invariant r == twoRowsResource(
+  //       slot_idx as nat, Info(Empty, RemoveTidying(rid, inital_key, found_value)),
+  //       NextPos(slot_idx as nat), Info(next_entry, Free),
+  //       0)
+  //     invariant handle.m == v.row_mutexes[slot_idx]
+  //     invariant next_handle.m == v.row_mutexes[NextPos(slot_idx as nat)]
+  //     decreases *
+  //   {
+  //     slot_idx' := getNextIndex(slot_idx);
 
-      if next_entry.Empty? || (next_entry.Full? && hash(next_entry.kv.key) == slot_idx') {
-        assert DoneTidying(r, slot_idx as nat);
-        break;
-      }
+  //     if next_entry.Empty? || (next_entry.Full? && hash(next_entry.kv.key) == slot_idx') {
+  //       assert DoneTidying(r, slot_idx as nat);
+  //       break;
+  //     }
 
-      ghost var r' := twoRowsResource(
-        slot_idx as nat, Info(next_entry, Free),
-        slot_idx' as nat, Info(Empty, RemoveTidying(rid, inital_key, found_value)),
-        0);
-      r := easy_transform_step(r, r', RemoveTidyStep(slot_idx as nat));
+  //     ghost var r' := twoRowsResource(
+  //       slot_idx as nat, Info(next_entry, Free),
+  //       slot_idx' as nat, Info(Empty, RemoveTidying(rid, inital_key, found_value)),
+  //       0);
+  //     r := easy_transform_step(r, r', RemoveTidyStep(slot_idx as nat));
 
-      ghost var left := oneRowResource(slot_idx' as nat, Info(Empty, RemoveTidying(rid, inital_key, found_value)), 0);
-      ghost var right := oneRowResource(slot_idx as nat, Info(next_entry, Free), 0);
+  //     ghost var left := oneRowResource(slot_idx' as nat, Info(Empty, RemoveTidying(rid, inital_key, found_value)), 0);
+  //     ghost var right := oneRowResource(slot_idx as nat, Info(next_entry, Free), 0);
 
-      r, rmutex := SSM.split(r, left, right);
-      v.row_mutexes[slot_idx].release(Row(next_entry, rmutex), handle);
+  //     r, rmutex := SSM.split(r, left, right);
+  //     v.row_mutexes[slot_idx].release(Row(next_entry, rmutex), handle);
 
-      slot_idx := slot_idx';
-      slot_idx' := getNextIndex(slot_idx);
-      handle := next_handle;
+  //     slot_idx := slot_idx';
+  //     slot_idx' := getNextIndex(slot_idx);
+  //     handle := next_handle;
 
-      next_row, next_handle := v.row_mutexes[slot_idx'].acquire();
-      linear var Row(next_entry', next_row_r) := next_row;
-      next_entry := next_entry';
-      r := SSM.join(r, next_row_r);
-    }
+  //     next_row, next_handle := v.row_mutexes[slot_idx'].acquire();
+  //     linear var Row(next_entry', next_row_r) := next_row;
+  //     next_entry := next_entry';
+  //     r := SSM.join(r, next_row_r);
+  //   }
 
-    assert DoneTidying(r, slot_idx as nat);
+  //   assert DoneTidying(r, slot_idx as nat);
 
-    slot_idx' := getNextIndex(slot_idx);
-    output := MapIfc.RemoveOutput(true);
+  //   slot_idx' := getNextIndex(slot_idx);
+  //   output := MapIfc.RemoveOutput(true);
 
-    linear var cap; glinear var cap_handle; var tid;
-    cap, cap_handle, tid := acquireCapacity(v, thread_id);
-    linear var AllocatorBin(count, cap_r) := cap;
-    r := SSM.join(r, cap_r);
+  //   linear var cap; glinear var cap_handle; var tid;
+  //   cap, cap_handle, tid := acquireCapacity(v, thread_id);
+  //   linear var AllocatorBin(count, cap_r) := cap;
+  //   r := SSM.join(r, cap_r);
 
-    r' := SSM.Variables(
-      twoRowsTable(slot_idx as nat, Info(Empty, Free), slot_idx' as nat, Info(next_entry, Free)),
-      count as nat + 1,
-      multiset{},
-      multiset{ Stub(rid, output) }
-    );
+  //   r' := SSM.Variables(
+  //     twoRowsTable(slot_idx as nat, Info(Empty, Free), slot_idx' as nat, Info(next_entry, Free)),
+  //     count as nat + 1,
+  //     multiset{},
+  //     multiset{ Stub(rid, output) }
+  //   );
 
-    step := RemoveDoneStep(slot_idx as nat);
-    r := easy_transform_step(r, r', step);
+  //   step := RemoveDoneStep(slot_idx as nat);
+  //   r := easy_transform_step(r, r', step);
 
-    ghost var left := SSM.Variables(
-      oneRowTable(slot_idx' as nat, Info(next_entry, Free)),
-      count as nat + 1,
-      multiset{},
-      multiset{ Stub(rid, output) });
-    ghost var right := oneRowResource(slot_idx as nat, Info(Empty, Free), 0);
+  //   ghost var left := SSM.Variables(
+  //     oneRowTable(slot_idx' as nat, Info(next_entry, Free)),
+  //     count as nat + 1,
+  //     multiset{},
+  //     multiset{ Stub(rid, output) });
+  //   ghost var right := oneRowResource(slot_idx as nat, Info(Empty, Free), 0);
 
-    r, rmutex := SSM.split(r, left, right);
-    v.row_mutexes[slot_idx].release(Row(Empty, rmutex), handle);
+  //   r, rmutex := SSM.split(r, left, right);
+  //   v.row_mutexes[slot_idx].release(Row(Empty, rmutex), handle);
 
-    r, rmutex := SSM.split(r, 
-      SSM.output_stub(rid, output).(insert_capacity := count as nat + 1), 
-      oneRowResource(slot_idx' as nat, Info(next_entry, Free), 0));
-    v.row_mutexes[slot_idx'].release(Row(next_entry, rmutex), next_handle);
+  //   r, rmutex := SSM.split(r, 
+  //     SSM.output_stub(rid, output).(insert_capacity := count as nat + 1), 
+  //     oneRowResource(slot_idx' as nat, Info(next_entry, Free), 0));
+  //   v.row_mutexes[slot_idx'].release(Row(next_entry, rmutex), next_handle);
 
-    r, cap_r := SSM.split(r,
-      SSM.output_stub(rid, output), 
-      unit().(insert_capacity := count as nat + 1));
+  //   r, cap_r := SSM.split(r,
+  //     SSM.output_stub(rid, output), 
+  //     unit().(insert_capacity := count as nat + 1));
   
-    assert CAP.BinInv(AllocatorBin(count as nat +1, cap_r)); // ha ha ha
-    v.allocator[tid].release(AllocatorBin(count+1, cap_r), cap_handle);
+  //   assert CAP.BinInv(AllocatorBin(count as nat +1, cap_r)); // ha ha ha
+  //   v.allocator[tid].release(AllocatorBin(count+1, cap_r), cap_handle);
 
-    out_sv := r;
-  }
+  //   out_sv := r;
+  // }
 
-  method doRemove(v: Variables, input: Ifc.Input, rid: int, thread_id: uint32, glinear in_sv: SSM.Variables)
-    returns (output: Ifc.Output, glinear out_sv: SSM.Variables)
-    decreases *
+  // method doRemove(v: Variables, input: Ifc.Input, rid: int, thread_id: uint32, glinear in_sv: SSM.Variables)
+  //   returns (output: Ifc.Output, glinear out_sv: SSM.Variables)
+  //   decreases *
 
-    requires Inv(v)
-    requires input.RemoveInput?
-    requires isInputResource(in_sv, rid, input)
-    ensures out_sv == SSM.output_stub(rid, output)
-  {
-    var query_ticket := Ticket(rid, input);
-    var key := input.key;
-    var hash_idx := hash(key); var slot_idx := hash_idx;
+  //   requires Inv(v)
+  //   requires input.RemoveInput?
+  //   requires isInputResource(in_sv, rid, input)
+  //   ensures out_sv == SSM.output_stub(rid, output)
+  // {
+  //   var query_ticket := Ticket(rid, input);
+  //   var key := input.key;
+  //   var hash_idx := hash(key); var slot_idx := hash_idx;
 
-    linear var row; glinear var handle;
-    row, handle := v.row_mutexes[slot_idx].acquire();
+  //   linear var row; glinear var handle;
+  //   row, handle := v.row_mutexes[slot_idx].acquire();
 
-    linear var Row(entry, row_r) := row;
-    glinear var r := SSM.join(in_sv, row_r);
+  //   linear var Row(entry, row_r) := row;
+  //   glinear var r := SSM.join(in_sv, row_r);
 
-    var slot_idx' :uint32;
-    glinear var rmutex;
+  //   var slot_idx' :uint32;
+  //   glinear var rmutex;
 
-    glinear var r' := oneRowResource(hash_idx as nat, Info(entry, Removing(rid, key)), 0);
-    var step : Step := ProcessRemoveTicketStep(query_ticket);
-    r := easy_transform_step(r, r', step);
+  //   glinear var r' := oneRowResource(hash_idx as nat, Info(entry, Removing(rid, key)), 0);
+  //   var step : Step := ProcessRemoveTicketStep(query_ticket);
+  //   r := easy_transform_step(r, r', step);
 
-    while true 
-      invariant Inv(v);
-      invariant 0 <= slot_idx < FixedSizeImpl();
-      invariant r == oneRowResource(slot_idx as nat, Info(entry, Removing(rid, key)), 0)
-      invariant step.RemoveNotFoundStep? ==> 
-        (entry.Full? && shouldHashGoBefore(hash_idx, hash(entry.kv.key), slot_idx))
-      invariant step.RemoveTidyStep? ==> (
-        && TidyEnabled(r, slot_idx as nat)
-        && KnowRowIsFree(r, NextPos(slot_idx as nat)))
-      invariant handle.m == v.row_mutexes[slot_idx]
-      decreases *
-    {
-      var slot_idx' := getNextIndex(slot_idx);
+  //   while true 
+  //     invariant Inv(v);
+  //     invariant 0 <= slot_idx < FixedSizeImpl();
+  //     invariant r == oneRowResource(slot_idx as nat, Info(entry, Removing(rid, key)), 0)
+  //     invariant step.RemoveNotFoundStep? ==> 
+  //       (entry.Full? && shouldHashGoBefore(hash_idx, hash(entry.kv.key), slot_idx))
+  //     invariant step.RemoveTidyStep? ==> (
+  //       && TidyEnabled(r, slot_idx as nat)
+  //       && KnowRowIsFree(r, NextPos(slot_idx as nat)))
+  //     invariant handle.m == v.row_mutexes[slot_idx]
+  //     decreases *
+  //   {
+  //     var slot_idx' := getNextIndex(slot_idx);
 
-      match entry {
-        case Empty => {
-          step := RemoveNotFoundStep(slot_idx as nat);
-        }
-        case Full(KV(entry_key, value)) => {
-          if entry_key == key {
-            step := RemoveFoundItStep(slot_idx as nat);
-          } else {
-            var should_go_before := shouldHashGoBefore(hash_idx, hash(entry_key), slot_idx);
+  //     match entry {
+  //       case Empty => {
+  //         step := RemoveNotFoundStep(slot_idx as nat);
+  //       }
+  //       case Full(KV(entry_key, value)) => {
+  //         if entry_key == key {
+  //           step := RemoveFoundItStep(slot_idx as nat);
+  //         } else {
+  //           var should_go_before := shouldHashGoBefore(hash_idx, hash(entry_key), slot_idx);
 
-            if !should_go_before {
-              step := RemoveSkipStep(slot_idx as nat);
-            } else {
-              step := RemoveNotFoundStep(slot_idx as nat);
-            }
-          }
-        }
-      }
+  //           if !should_go_before {
+  //             step := RemoveSkipStep(slot_idx as nat);
+  //           } else {
+  //             step := RemoveNotFoundStep(slot_idx as nat);
+  //           }
+  //         }
+  //       }
+  //     }
 
-      if step.RemoveNotFoundStep? || step.RemoveFoundItStep? {
-        break;
-      }
+  //     if step.RemoveNotFoundStep? || step.RemoveFoundItStep? {
+  //       break;
+  //     }
 
-      linear var next_row; glinear var next_handle;
-      next_row, next_handle := v.row_mutexes[slot_idx'].acquire();
-      linear var Row(next_entry, next_row_r) := next_row;
-      r := SSM.join(r, next_row_r);
+  //     linear var next_row; glinear var next_handle;
+  //     next_row, next_handle := v.row_mutexes[slot_idx'].acquire();
+  //     linear var Row(next_entry, next_row_r) := next_row;
+  //     r := SSM.join(r, next_row_r);
 
-      r' := twoRowsResource(slot_idx as nat, Info(entry, Free), slot_idx' as nat, Info(next_entry, Removing(rid, key)), 0);
-      r := easy_transform_step(r, r', step);
+  //     r' := twoRowsResource(slot_idx as nat, Info(entry, Free), slot_idx' as nat, Info(next_entry, Removing(rid, key)), 0);
+  //     r := easy_transform_step(r, r', step);
 
-      ghost var left := oneRowResource(slot_idx' as nat, Info(next_entry, Removing(rid, key)), 0);
-      ghost var right := oneRowResource(slot_idx as nat, Info(entry, Free), 0);
-      r, rmutex := SSM.split(r, left, right);
-      v.row_mutexes[slot_idx].release(Row(entry, rmutex), handle);
+  //     ghost var left := oneRowResource(slot_idx' as nat, Info(next_entry, Removing(rid, key)), 0);
+  //     ghost var right := oneRowResource(slot_idx as nat, Info(entry, Free), 0);
+  //     r, rmutex := SSM.split(r, left, right);
+  //     v.row_mutexes[slot_idx].release(Row(entry, rmutex), handle);
 
-      slot_idx := slot_idx';
-      entry := next_entry;
-      handle := next_handle;
-    }
+  //     slot_idx := slot_idx';
+  //     entry := next_entry;
+  //     handle := next_handle;
+  //   }
 
-    if step.RemoveNotFoundStep? {
-      output := MapIfc.RemoveOutput(false);
-      r' := SSM.Variables(oneRowTable(slot_idx as nat, Info(entry, Free)), 0, multiset{}, multiset{Stub(rid, output)}); 
-      r := easy_transform_step(r, r', step);
-      ghost var left := SSM.output_stub(rid, output);
-      ghost var right := oneRowResource(slot_idx as nat, Info(entry, Free), 0);
-      r, rmutex := SSM.split(r, left, right);
-      v.row_mutexes[slot_idx].release(Row(entry, rmutex), handle);
-    } else {
-      output, r := doRemoveFound(v, rid, slot_idx, hash_idx, key, entry, thread_id, handle, r);
-    }
+  //   if step.RemoveNotFoundStep? {
+  //     output := MapIfc.RemoveOutput(false);
+  //     r' := SSM.Variables(oneRowTable(slot_idx as nat, Info(entry, Free)), 0, multiset{}, multiset{Stub(rid, output)}); 
+  //     r := easy_transform_step(r, r', step);
+  //     ghost var left := SSM.output_stub(rid, output);
+  //     ghost var right := oneRowResource(slot_idx as nat, Info(entry, Free), 0);
+  //     r, rmutex := SSM.split(r, left, right);
+  //     v.row_mutexes[slot_idx].release(Row(entry, rmutex), handle);
+  //   } else {
+  //     output, r := doRemoveFound(v, rid, slot_idx, hash_idx, key, entry, thread_id, handle, r);
+  //   }
 
-    out_sv := r;
-  }
+  //   out_sv := r;
+  // }
 
-  method call(v: Variables, input: Ifc.Input, rid: int, glinear in_sv: SSM.Variables, thread_id: uint32)
-    returns (output: Ifc.Output, glinear out_sv: SSM.Variables)
-    decreases *
-  // requires Inv(o)
-  // requires ticket == SSM.input_ticket(rid, key)
-    ensures out_sv == SSM.output_stub(rid, output)
-  {
-    // Find the ticket.
-    assert |in_sv.tickets| == 1;
-    var the_ticket :| the_ticket in in_sv.tickets;
+  // method call(v: Variables, input: Ifc.Input, rid: int, glinear in_sv: SSM.Variables, thread_id: uint32)
+  //   returns (output: Ifc.Output, glinear out_sv: SSM.Variables)
+  //   decreases *
+  // // requires Inv(o)
+  // // requires ticket == SSM.input_ticket(rid, key)
+  //   ensures out_sv == SSM.output_stub(rid, output)
+  // {
+  //   // Find the ticket.
+  //   assert |in_sv.tickets| == 1;
+  //   var the_ticket :| the_ticket in in_sv.tickets;
 
-    if the_ticket.input.QueryInput? {
-      output, out_sv := doQuery(v, input, rid, in_sv);
-    } else if the_ticket.input.InsertInput? {
-      output, out_sv := doInsert(v, input, rid, thread_id, in_sv);
-    } else if the_ticket.input.RemoveInput? {
-      output, out_sv := doRemove(v, input, rid, thread_id, in_sv);
-    } else {
-      out_sv := in_sv;
-      assert false;
-    }
-  }
+  //   if the_ticket.input.QueryInput? {
+  //     output, out_sv := doQuery(v, input, rid, in_sv);
+  //   } else if the_ticket.input.InsertInput? {
+  //     output, out_sv := doInsert(v, input, rid, thread_id, in_sv);
+  //   } else if the_ticket.input.RemoveInput? {
+  //     output, out_sv := doRemove(v, input, rid, thread_id, in_sv);
+  //   } else {
+  //     out_sv := in_sv;
+  //     assert false;
+  //   }
+  // }
 
-  lemma NewTicket_RefinesMap(s: SSM.Variables, s': SSM.Variables, rid: int, input: Ifc.Input)
-  {
-  }
+  // lemma NewTicket_RefinesMap(s: SSM.Variables, s': SSM.Variables, rid: int, input: Ifc.Input)
+  // {
+  // }
   
-  lemma ReturnStub_RefinesMap(s: SSM.Variables, s': SSM.Variables, rid: int, output: Ifc.Output)
-  {
-  }
+  // lemma ReturnStub_RefinesMap(s: SSM.Variables, s': SSM.Variables, rid: int, output: Ifc.Output)
+  // {
+  // }
   
 }
